lock-coupling unfinished

flows.v
@@ -77,12 +77,15 @@ Proof. Admitted.
 Type 1%Qp.
 
 (* This is the rule AUTH-FI-UPD in the paper *)
-Definition flowint_update_P (I I_n I_n': flowintUR) (x : auth flowintUR) : Prop := True.
-(*  match auth_auth_proj x with
-  | Some ( Qp_one , {| agree_car := [I']; agree_not_nil := eq_refl |}) => I_n' = auth_frag_proj x ∧ contextualLeq I I' ∧ ∃ I_o, I = I_n ⋅ I_o ∧ I' = I_n' ⋅ I_o
+Definition flowint_update_P (I I_n I_n': flowintUR) (x : authR flowintUR) : Prop :=
+  match (auth_auth_proj x) with
+  | Some (Qp_one, {| agree_car := [I']; agree_not_nil := eq_refl |}) => (I_n' = auth_frag_proj x) 
+                                                      ∧ contextualLeq I I' ∧ ∃ I_o, I = I_n ⋅ I_o ∧ I' = I_n' ⋅ I_o
+  | Some (q, _) => False
   | _ => False
   end.
-*)
+
+
 Lemma flowint_update I I_n I_n' :
   contextualLeq I_n I_n' → (● I ⋅ ◯ I_n) ~~>: (flowint_update_P I I_n I_n').
 Proof. Admitted.
