give-up.v
@@ -1,5 +1,3 @@
-(*  1) what to keep outside (persistant stuff)
-*)
 Add LoadPath "/home/nisarg/Academics/templates".
 From iris.algebra Require Import excl auth gmap agree gset.
 From iris.heap_lang Require Export lifting notation locations lang.
@@ -9,7 +7,7 @@ From iris.proofmode Require Import tactics.
 From iris.heap_lang Require Import proofmode notation par.
 From iris.bi.lib Require Import fractional.
 From iris.bi Require Import derived_laws_sbi.
-Require Import flows.
+Require Export flows.
 Set Default Proof Using "Type*".
 
 (* ---------- The program ---------- *)
@@ -22,6 +20,7 @@ Variable decisiveOp : (dOp → val).
 Variable searchStrSpec : (dOp → val).
 Variable lockLoc : node → loc.
 Variable getLockLoc : val.
+
 
 Variable in_inset : key → flowintUR → node → Prop.                    (* Couldn't load from flows.v *)
 Variable in_edgeset : key → flowintUR → node → node → Prop.
@@ -80,8 +79,8 @@ Instance subG_nodesetΣ {Σ} : subG nodesetΣ Σ → nodesetG Σ.
 Proof. solve_inG. Qed.
 
 (* RA for set of contents *)
-Class contentG Σ := ContentG { content_inG :> inG Σ (gsetR key) }.
-Definition contentΣ : gFunctors := #[GFunctor (gsetR key)].
+Class contentG Σ := ContentG { content_inG :> inG Σ (authR (optionUR (exclR (gsetR key)))) }.
+Definition contentΣ : gFunctors := #[GFunctor (authR (optionUR (exclR (gsetR key))))].
 
 Instance subG_contentΣ {Σ} : subG contentΣ Σ → contentG Σ.
 Proof. solve_inG. Qed.
@@ -89,9 +88,8 @@ Proof. solve_inG. Qed.
 Section Give_Up_Template.
   Context `{!heapG Σ, !flowintG Σ, !nodesetG Σ, !contentG Σ} (N : namespace).
   Notation iProp := (iProp Σ).
-  Variable (Δ : list (prodO valO valO -n> iProp)).
 
-  (* ---------- Flow interface set-up specific to this proof ---------- *)
+(* ---------- Flow interface set-up specific to this proof ---------- *)
 
   Variable root : node.
   Variable hrep : node → flowintUR → iProp.
@@ -136,25 +134,15 @@ Section Give_Up_Template.
       destruct H as ((HC1 & HkC1) & (HC2 & HkC2) & HEq); congruence.
   Qed.
 
-(*  Axiom cg_decisive_op_spec :
-    ∀ dop Γ K E t τ C γ_c k,
-    (own γ_c C -∗                                   (* Precondition *)
-     (∀ res C', own γ_c C' ∗ Ψ dop k C C' res -∗    (* Postcondition *)
-      ({E;Δ;Γ} ⊨ t ≤log≤ fill K (#res) : τ)) -∗
-     {E;Δ;Γ} ⊨ t ≤log≤ fill K (searchStrSpec dop #k) : τ)%I.
-
-To add what is needed later.
-*)
-
-  Axiom Ψ_keyset_theorem : ∀ dop k n I_n I_n' I I' res,
+  Axiom Ψ_keyset_theorem : ∀ (dop: dOp) (k: key) (n: node) (I_n I_n' I I': flowintUR) (res: bool),
       ⌜globalint I⌝ ∗ ⌜Nds I_n = {[n]}⌝ ∗ ⌜in_inset k I_n n⌝ ∗ ⌜not_in_outset k I_n n⌝
-      ∗ ⌜(∃ I_o, I = I_n ⋅ I_o ∧ I' = I_n' ⋅ I_o)⌝ ∗ ✓ I ∗ ✓ I'
-      -∗ Ψ dop k (cont I_n) (cont I_n') res -∗ Ψ dop k (cont I) (cont I') res.
+      ∗ ⌜(∃ (I_o: flowintUR), I = I_n ⋅ I_o ∧ I' = I_n' ⋅ I_o)⌝ ∗ ✓ I ∗ ✓ I'
+      -∗ Ψ dop k (cont I_n) (cont I_n') res -∗ ⌜Ψ dop k (cont I) (cont I') res⌝.
 
 
   (* ---------- Helper functions specs - proved for each implementation in GRASShopper ---------- *)
 
-Parameter getLockLoc_spec : ∀ (n: node),
+  Parameter getLockLoc_spec : ∀ (n: node),
                   (<<< True >>> getLockLoc #n @ ⊤
                            <<< ∃ l:loc, ⌜lockLoc n = l⌝, RET #l >>>)%I.
 
@@ -172,10 +160,10 @@ Parameter getLockLoc_spec : ∀ (n: node),
                                                     false => NONEV end) >>>)%I.
 
   Parameter decisiveOp_spec : ∀ (dop: dOp) (I_n: flowintUR) (n: node) (k: key),
-                  (<<< hrep n I_n ∗ ⌜in_inset k I_n n⌝ ∗ ⌜not_in_outset k I_n n⌝ >>>
+                  (<<< hrep n I_n ∗ ⌜in_inset k I_n n⌝ ∗ ⌜not_in_outset k I_n n⌝ ∗ ⌜Nds I_n = {[n]}⌝ >>>
                         decisiveOp dop #n #k @ ⊤
                    <<< ∃ (b: bool) (I_n': flowintUR) (res: bool), match b with false => hrep n I_n |
-                                                                         true => hrep n I_n' ∗ Ψ dop k (cont I_n) (cont I_n') res
+                                                                         true => hrep n I_n' ∗ ⌜Ψ dop k (cont I_n) (cont I_n') res⌝
                                                                                 ∗ ⌜contextualLeq I_n I_n'⌝ ∗ ⌜Nds I_n' = {[n]}⌝ end,
                        RET (match b with false => NONEV |
                                          true => (SOMEV #res) end) >>>)%I. 
@@ -198,7 +186,7 @@ Parameter getLockLoc_spec : ∀ (n: node),
 
   Definition main_inv (γ: gname) (γ_fp: gname) (γ_c: gname) I Ns C
     : iProp :=
-    (own γ_c C ∗ ⌜C = cont I⌝
+    (own γ_c (● (Some (Excl C))) ∗ ⌜C = cont I⌝
         ∗ own γ (● I) ∗ ⌜globalint I⌝
         ∗ ([∗ set] n ∈ (Nds I), (∃ b: bool, (lockLoc n) ↦ #b
                                 ∗ if b then True else (∃ (In: flowintUR),
@@ -235,13 +223,51 @@ Parameter getLockLoc_spec : ∀ (n: node),
     rewrite -own_op. rewrite own_valid. iPureIntro. rewrite auth_valid_discrete.
     simpl. rewrite ucmra_unit_left_id_L. Admitted.
 
+  Lemma auth_agree γ xs ys :
+    own γ (● (Excl' xs)) -∗ own γ (◯ (Excl' ys)) -∗ ⌜xs = ys⌝.
+  Proof.
+   iIntros "Hγ● Hγ◯". by iDestruct (own_valid_2 with "Hγ● Hγ◯")
+      as %[<-%Excl_included%leibniz_equiv _]%auth_both_valid.
+  Qed.
+
+  (** The view of the authority can be updated together with the local view. *)
+  Lemma auth_update γ ys xs1 xs2 :
+    own γ (● (Excl' xs1)) -∗ own γ (◯ (Excl' xs2)) ==∗
+      own γ (● (Excl' ys)) ∗ own γ (◯ (Excl' ys)).
+  Proof.
+    iIntros "Hγ● Hγ◯".
+    iMod (own_update_2 _ _ _ (● Excl' ys ⋅ ◯ Excl' ys)
+      with "Hγ● Hγ◯") as "[$$]".
+    { by apply auth_update, option_local_update, exclusive_local_update. }
+    done.
+  Qed.
+
+
   Lemma flowint_update_result γ I I_n I_n' x :
     ⌜flowint_update_P I I_n I_n' x⌝ ∧ own γ x -∗
                                           ∃ I', ⌜contextualLeq I I'⌝ ∗ ⌜∃ I_o, I = I_n ⋅ I_o ∧ I' = I_n' ⋅ I_o⌝ 
                                                                      ∗ own γ (● I' ⋅ ◯ I_n').
-  Proof. Admitted.
-(* flowint_update_P is undefined
+  Proof.
+    unfold flowint_update_P. simpl.
+    case_eq (auth_auth_proj x); last first.
+    - intros H. iIntros "(% & ?)". iExFalso. done.
+    - intros p. intros H. case_eq p. intros q a Hp. case_eq a.
+      intros intl b Ha. destruct intl as [ | I' ?]. iIntros "(% & ?)". iExFalso. done.
+      case_eq intl; last first. intros u0 l _. iIntros "(% & ?)". iExFalso. done.
+      + intros Hintl. simpl in b. assert (b = eq_refl) as H0. { admit. }
+        rewrite H0. iIntros "(Hfr & Hown)". iDestruct "Hfr" as %Hfr. destruct Hfr as [Hfrag Hcon].
+        destruct Hcon as [Hcon HIo]. destruct HIo as [Io HIo]. iExists I'.
+        iSplitR. iPureIntro. { admit. }
+        iSplitR. iPureIntro. exists Io. done.
+  Admitted.
+(*    unfold flowint_update_P. simpl.
+    case_eq x. simpl. case_eq (Some (Qp_one, {| agree_car := [x]; agree_not_nil := eq_refl |})). simpl.
+    - intros e Hax xa xo Hx.
+      case_eq e.
+      + intros u He. rewrite <-Hx.
+    iIntros "H". *)
 
+(* 
     unfold flowint_update_P. simpl.
     case_eq x.
     case_eq (● x).
@@ -308,17 +334,17 @@ Parameter getLockLoc_spec : ∀ (n: node),
           * wp_pures. done.
   Qed.
 
-  Lemma unlockNode_spec (γ: gname) (γ_fp: gname) (γ_c: gname) (n: node) (Ns: gset node) (I_n: flowintUR) :
-    is_dict γ γ_fp γ_c -∗ own γ_fp (◯ Ns) ∗ ⌜n ∈ Ns⌝ ∗ ⌜Nds I_n = {[n]}⌝ -∗
-          <<< hrep n I_n ∗ own γ (◯ I_n) >>>
+  Lemma unlockNode_spec (γ: gname) (γ_fp: gname) (γ_c: gname) (n: node) (Ns: gset node) :
+    is_dict γ γ_fp γ_c -∗ own γ_fp (◯ Ns) ∗ ⌜n ∈ Ns⌝ -∗
+          <<< ∀ (I_n: flowintUR), hrep n I_n ∗ own γ (◯ I_n) ∗ ⌜Nds I_n = {[n]}⌝ >>>
                 unlockNode #n    @ ⊤ ∖ ↑dictN
           <<< True, RET #() >>>.
   Proof.
-    iIntros "#Hinv (Hfp & Hin & Hnds)" (Φ) "AU". wp_lam. awp_apply getLockLoc_spec.
+    iIntros "#Hinv (Hfp & Hin)" (Φ) "AU". wp_lam. awp_apply getLockLoc_spec.
     iAssert (True)%I as "Ht". done.
     iAaccIntro with "Ht". eauto 4 with iFrame.
-    iIntros (l) "#Hl". iModIntro. wp_let. iInv dictN as ">HI".
-    iDestruct "HI" as (I' N' C') "(H1 & H2 & H3 & H4 & H5 & H6 & H7)".  iDestruct "Hl" as %Hl.
+    iIntros (l) "Hl". iDestruct "Hl" as %Hl. iModIntro. wp_let. iInv dictN as ">HI".
+    iDestruct "HI" as (I' N' C') "(H1 & H2 & H3 & H4 & H5 & H6 & H7)".
     iAssert (⌜n ∈ Nds I'⌝)%I with "[Hfp Hin H6 H7]" as "%".
     { (*iEval (rewrite <- H1).*) iPoseProof ((auth_set_incl γ_fp Ns N') with "[$]") as "%".
       iDestruct "H7" as %H7. iDestruct "Hin" as %Hl2. iEval (rewrite <-H7). iPureIntro. set_solver. }
@@ -326,22 +352,23 @@ Parameter getLockLoc_spec : ∀ (n: node),
     iDestruct "H5" as "[ho hoho]".
     iDestruct "ho" as (b) "[Hlock Hlock']".
     iEval (rewrite Hl) in "Hlock".
-    iMod "AU" as "[[Hrep Hs] [_ Hcl]]". wp_store.
+    iMod "AU" as (I_n) "[Hr [_ Hcl]]". wp_store.
     iAssert (True)%I as "Ht". done.
     iMod ("Hcl" with "Ht") as "HΦ".
     iModIntro. iModIntro. iSplitR "HΦ". iNext. iExists I', N', C'. rewrite /main_inv. iFrame.
-    iApply "hoho". iExists false. iEval (rewrite <-Hl) in "Hlock". iFrame. iExists I_n. iFrame. done.
+    iApply "hoho". iExists false. iEval (rewrite <-Hl) in "Hlock". iFrame. iExists I_n. 
+    iDestruct "Hr" as "(? & ? & ?)". eauto with iFrame. done.
   Qed.
 
 
   (* ---------- Ghost state manipulation to make final proof cleaner ---------- *)
 
   Lemma ghost_update_step γ γ_fp γ_c (n n': node) (k:key) (Ns: gset node) (I_n: flowintUR):
-          is_dict γ γ_fp γ_c ∗ own γ_fp (◯ Ns) ∗ ⌜n ∈ Ns⌝ ∗ own γ (◯ I_n) ∗ ⌜Nds I_n = {[n]}⌝
+          is_dict γ γ_fp γ_c -∗ own γ_fp (◯ Ns) ∗ ⌜n ∈ Ns⌝ ∗ own γ (◯ I_n) ∗ ⌜Nds I_n = {[n]}⌝
        ∗ ⌜in_inset k I_n n⌝ ∗ ⌜in_edgeset k I_n n n'⌝ ={ ⊤ }=∗ ∃ (Ns': gset node), own γ_fp (◯ Ns') ∗ ⌜n' ∈ Ns'⌝ 
-                                                        ∗ ⌜root ∈ Ns'⌝.
-  Proof. 
-    iIntros "(Hinv & HNs & % & HIn & % & % & %)".
+                                                        ∗ own γ (◯ I_n) ∗ ⌜root ∈ Ns'⌝.
+  Proof.
+    iIntros "#Hinv (HNs & % & HIn & % & % & %)".
     iInv dictN as ">HInv" "Hclose".
     iDestruct "HInv" as (I Ns' C) "HInv".
     iPoseProof (inv_impl_fp n Ns with "[$HInv $HNs //]") as "%".
@@ -361,61 +388,8 @@ Parameter getLockLoc_spec : ∀ (n: node),
     rewrite <-H6 in H8. iSplit. iPureIntro. done.
     iPureIntro. rewrite H6. apply globalint_root_fp. done.
   Admitted.
-    
-  
-(*
-  Lemma ghost_update_step γ γ_fp γ_c n n' (k: key) (Ns: gsetUR node) I_n Γ t t' τ :
-    is_dict γ γ_fp γ_c
-        ∗ own γ_fp (◯ Ns) ∗ ⌜n ∈ Ns⌝ ∗ own γ (◯ I_n) ∗ ⌜FP I_n = {[n]}⌝
-        ∗ ⌜in_inset k I_n n⌝ ∗ ⌜in_edgeset k I_n n n'⌝
-     -∗ ((∀ Ns', own γ_fp (◯ Ns') ∗ ⌜n' ∈ Ns'⌝ ∗ ⌜root ∈ Ns'⌝ ∗ own γ (◯ I_n)
-                 -∗ ({Δ;Γ} ⊨ t ≤log≤ t' : τ))
-           -∗ {Δ;Γ} ⊨ t ≤log≤ t' : τ)%I.
-  Proof.
-    iIntros "(Hinv & HNs & % & HIn & % & % & %) HPost".
-    iInv dictN as ">HInv" "HClose".
-    iDestruct "HInv" as (I Ns' C) "HInv".
-    iPoseProof (inv_impl_fp n Ns with "[$HInv $HNs //]") as "%".
-    (* I = I_n ⋅ I2 *)
-    iDestruct "HInv" as "(? & % & HI & % & ? & HNs' & %)".
-    iPoseProof (auth_own_incl with "[$HI $HIn]") as "%".
-    unfold included in H8. destruct H8 as [I2 Hmult].
-    (* n' ∈ FP I *)
-    iPoseProof ((own_valid γ (● I)) with "HI") as "%".
-    iAssert (⌜n' ∈ FP I⌝)%I as "%".
-    { iPureIntro.
-      assert (n' ∈ FP I2).
-      { apply (flowint_step I I_n _ k n). done.
-        by apply auth_auth_valid.
-        replace (FP I_n). set_solver. done. by apply globalint_fpo. }
-      apply flowint_comp_fp in Hmult. set_solver.
-    }
-    (* snapshot fp to get Ns' *)
-    iMod (own_update γ_fp (● Ns') (● Ns' ⋅ ◯ Ns') with "HNs'") as "HNs'";
-      first by apply auth_set_snapshot.
-    iEval (rewrite own_op) in "HNs'". iDestruct "HNs'" as "(HNs0 & HNs')".
 
-    iMod ("HClose" with "[-HPost HNs' HIn]").
-    {
-      iNext. iExists I, Ns', C. iFrame "# % ∗".
-    }
-    iApply ("HPost" with "[-]").
-    iFrame. iPureIntro. split; replace Ns'; try done.
-    by apply globalint_root_fp.
-  Qed.
-*)
   (* ---------- Refinement proofs ---------- *)
-
-(*  Lemma traverse_spec (γ: gname) (γ_fp: gname) γ_c (Ns: gsetUR node)
-        Γ K t τ (n: node) (k: key) :
-    is_dict γ γ_fp γ_c -∗
-    (own γ_fp (◯ Ns) ∗ ⌜n ∈ Ns⌝ ∗ ⌜root ∈ Ns⌝ -∗
-     (∀ (n': node) (Ns': gsetUR node) (I_n': flowintUR),
-       own γ_fp (◯ Ns') ∗ ⌜n' ∈ Ns'⌝ ∗ own γ (◯ I_n') ∗ hrep n' I_n' ∗ ⌜FP I_n' = {[n']}⌝
-       ∗ ⌜in_inset k I_n' n'⌝ ∗ ⌜not_in_outset k I_n' n'⌝ -∗
-       ({Δ;Γ} ⊨ fill K (#n') ≤log≤ t : τ)) -∗
-     {Δ;Γ} ⊨ fill K (traverse root #n #k) ≤log≤ t : τ)%I.
-*)
 
   Lemma traverse_spec (γ γ_fp γ_c: gname) (k: key) :
         ∀ (n: node) (Ns: gsetUR node),
@@ -426,7 +400,7 @@ Parameter getLockLoc_spec : ∀ (n: node),
           <<< ∃ (n': node) (Ns': gsetUR node) (I_n': flowintUR), ⌜n' ∈ Ns'⌝ ∗ own γ_fp (◯ Ns')
                  ∗ own γ (◯ I_n') ∗ hrep n' I_n' ∗ ⌜Nds I_n' = {[n']}⌝ 
                  ∗ ⌜in_inset k I_n' n'⌝ ∗ ⌜not_in_outset k I_n' n'⌝, RET #n' >>>.
-  Proof. 
+  Proof.
     iIntros (n Ns). iIntros "#HInv H". iLöb as "IH" forall (n Ns).
     iIntros (Φ) "AU". iDestruct "H" as "(#Hfp & #Hin & #Hr)".
     wp_lam. wp_let. awp_apply (lockNode_spec γ γ_fp γ_c n Ns).
@@ -441,47 +415,148 @@ Parameter getLockLoc_spec : ∀ (n: node),
           iAaccIntro with "Hrep". eauto with iFrame. iIntros (b n') "(Hrep & H2)". 
           destruct b.
             * (* findNext succeeds *) 
-               iModIntro. wp_pures. awp_apply (unlockNode_spec γ γ_fp γ_c n Ns In).
-               { done. } { eauto with iFrame. } iCombine "Hrep" "HInt" as "Haac".
-               iAaccIntro with "Haac". { iIntros "(Hrep & HInt)". iModIntro. iFrame. } iIntros "Ht". iModIntro.
-               wp_pures. iApply "IH". (*iMod ghost_update_step.*) admit. done.
+               iModIntro. wp_pures.
+               iDestruct (ghost_update_step γ γ_fp γ_c n n' k Ns In with "[HInv] [Hfp Hin HInt Hdom H1 H2]") as ">hoho".
+               { done. } { eauto with iFrame. } iDestruct "hoho" as (Ns') "(#Hfp' & #Hin' & HInt & #Hr')".
+               awp_apply (unlockNode_spec γ γ_fp γ_c n Ns).
+               { done. } { eauto with iFrame. }
+               iAssert (hrep n In ∗ own γ (◯ In) ∗ ⌜Nds In = {[n]}⌝)%I with "[Hrep HInt Hdom]" as "Haac". { eauto with iFrame. }
+               iAaccIntro with "Haac". { iIntros "(Hrep & HInt & HNds)". iModIntro. iFrame. } iIntros "Ht".
+               iModIntro. wp_pures. iSpecialize ("IH" $! n' Ns'). iApply "IH". eauto with iFrame. done.
             * (* findNext fails *)
               iMod "AU" as "[Ht [_ HClose]]". iSpecialize ("HClose" $! n Ns In).
               iMod ("HClose" with "[Hfp HInt Hrep Hdom H1 H2]") as "HΦ". eauto with iFrame.
               iModIntro. wp_pures. done.
         + (*inRange fails *)                                 (* Don't understand how the context is broken up with intro *)
-          wp_if. awp_apply (unlockNode_spec γ γ_fp γ_c n Ns In). done. eauto with iFrame.  iCombine "Hrep" "HInt" as "Haac".
-          iAaccIntro with "Haac". { iIntros "(Hrep & HInt)". iModIntro. iFrame. } 
+          wp_if. awp_apply (unlockNode_spec γ γ_fp γ_c n Ns). done. eauto with iFrame.
+          iAssert (hrep n In ∗ own γ (◯ In) ∗ ⌜Nds In = {[n]}⌝)%I with "[Hrep HInt Hdom]" as "Haac". { eauto with iFrame. }
+          iAaccIntro with "Haac". { iIntros "(Hrep & HInt & HNds)". iModIntro. iFrame. }
           iIntros. iModIntro. wp_pures. iApply "IH". eauto with iFrame. done.
-  Admitted.
+  Qed.
 
   Theorem searchStrOp_spec (γ γ_fp γ_c: gname) (dop: dOp) (k: key):
-          ∀ (Ns: gsetUR node) (C: gsetUR key),
-          is_dict γ γ_fp γ_c -∗ own γ_fp (◯ Ns) ∗ ⌜ root ∈ Ns ⌝ ∗ own γ_c (◯ C) -∗
-      <<< True >>>
+          ∀ (Ns: gsetUR node) (C: gset key),
+          is_dict γ γ_fp γ_c -∗ own γ_fp (◯ Ns) ∗ ⌜ root ∈ Ns ⌝ -∗
+      <<< own γ_c (◯ (Some (Excl C))) >>>
             (searchStrOp dop root) #k
                   @ ⊤∖↑dictN
-      <<< ∃ (C': gsetUR key) (res: bool), own γ_c (◯ C') ∗ Ψ dop k C C' res, RET #res >>>.
+      <<< ∃ (C': gset key) (res: bool), own γ_c (◯ (Some (Excl C'))) ∗ ⌜Ψ dop k C C' res⌝, RET #res >>>.
   Proof.
     iIntros (Ns C). iIntros "#HInv H" (Φ) "AU". iLöb as "IH" forall (Ns).
-    wp_lam. wp_bind(traverse _ _ _)%E. iDestruct "H" as "#(H1 & H2 &H3)".
+    wp_lam. wp_bind(traverse _ _ _)%E. iDestruct "H" as "#(H1 & H2)".
     awp_apply (traverse_spec γ γ_fp γ_c). done. eauto with iFrame.
     iAssert (True)%I as "Ht". done. iAaccIntro with "Ht". eauto with iFrame.
     iIntros (n Ns' In) "(#Hin & #Hfp & HInt & Hrep & #HNds & #Hinset & #Hout)". iModIntro. wp_let.
     wp_bind(decisiveOp dop _ _)%E. awp_apply (decisiveOp_spec dop In n k).
-    iAssert (⌜in_inset k In n⌝ ∗ ⌜not_in_outset k In n⌝)%I as "Haac1". { eauto with iFrame. }
-    iCombine "Hrep" "Haac1" as "Haac".
+    iAssert (hrep n In ∗ ⌜in_inset k In n⌝ ∗ ⌜not_in_outset k In n⌝ ∗ ⌜Nds In = {[n]}⌝)%I with "[Hrep Hinset Hout HNds]" as "Haac".
+    { eauto with iFrame. }
     iAaccIntro with "Haac". { iIntros "(Hrep & ?)". iModIntro. iFrame. }
-    iIntros (b In' res) "Hb". destruct b.
-    - iMod "AU" as "[Ht [_ Hcl]]". iDestruct "Hb" as "(Hf & H4 & H5 & H6)".
-      iSpecialize ("Hcl" $! (cont In') res). iAssert (⌜C = cont In⌝)%I as %Hcont. { admit. }
-      iEval (rewrite Hcont) in "H3". iEval (rewrite Hcont) in "Hcl". iMod ("Hcl" with "[H3 H4]"). wp_pures. iDestruct "Hb" as "(Hf & H4 & H5 & H6)". iMod "AU" as "[Ht [_ Hcl]]".
-      wp_bind(unlockNode _)%E. 
-      awp_apply (unlockNode_spec γ γ_fp γ_c n Ns' In').
-    - iModIntro. wp_pures. awp_apply (unlockNode_spec γ γ_fp γ_c n Ns' In). done. iSplit. done. iSplit. done. done.
-      iAaccIntro with "[$Hb $HInt]". iIntros "(Hb & HInt)". eauto with iFrame. iIntros. iModIntro.
-      wp_pures. iApply "IH". iSplit. iApply "H1". iSplit. done. done. done.
-f
+    iIntros (b In' result) "Hb". destruct b; last first.
+    - iModIntro. wp_pures. awp_apply (unlockNode_spec γ γ_fp γ_c n Ns'). done. iSplit. done. iApply "Hin".
+      iAssert (hrep n In ∗ own γ (◯ In) ∗ ⌜Nds In = {[n]}⌝)%I with "[Hb HInt HNds]" as "Haac". { eauto with iFrame. }
+      iAaccIntro with "Haac". iIntros "(Hb & HInt & _)". eauto with iFrame. iIntros. iModIntro.
+      wp_pures. iApply "IH". iSplit. iApply "H1". done. done.
+    - iInv dictN as ">HI". iDestruct "HI" as (I Nd Cs) "(H3 & H4 & H5 & H6 & H7 & H8 & H9)".
+      iDestruct "H4" as %H4. iEval (rewrite H4) in "H3".
+      iPoseProof (auth_own_incl with "[$H5 $HInt]") as (I2)"%".
+      iPoseProof ((own_valid γ (● I)) with "H5") as "%".
+      iDestruct "Hb" as "(Hrep & #Hdop & Hctx & HNds')". iDestruct "Hctx" as %Hctx.
+      iMod (own_updateP (flowint_update_P I In In') γ (● I ⋅ ◯ In) with "[H5 HInt]") as (?) "H0".
+      { apply (flowint_update I In In'). admit. } { rewrite own_op. iFrame. }
+      iPoseProof ((flowint_update_result γ I In In') with "H0") as (I') "(% & % & HIIn)".
+      iAssert (own γ (● I') ∗ own γ (◯ In'))%I with "[HIIn]" as "(HI' & HIn')". { by rewrite own_op. }
+      iPoseProof ((own_valid γ (● I')) with "HI'") as "%".
+      iPoseProof ((Ψ_keyset_theorem dop k n In In' I I' result) with "[H6 HNds Hinset Hout] [Hdop]") as "HΨI".
+      { repeat iSplitL; try done; iPureIntro; apply auth_auth_valid; done. } { done. }
+      iMod "AU" as "[hoho [_ Hcl]]". 
+      iDestruct (auth_agree with "H3 hoho") as %Hauth.
+      iMod (auth_update γ_c (cont I') with "H3 hoho") as "[H3 hoho]".
+      iSpecialize ("Hcl" $! (cont I') result). iEval (rewrite <-Hauth) in "Hcl".
+      iMod ("Hcl" with "[hoho HΨI]") as "HΦ". eauto with iFrame.
+      iModIntro. iSplitR "Hrep HIn' HNds HΦ".
+        + iNext. iExists I', Nd, (cont I').
+          unfold main_inv. assert (globalint I') as HI'. { (* by apply (contextualLeq_impl_globalint I I')*) admit. }
+          assert (Nds I = Nds I') as HH. { (*by apply (contextualLeq_impl_fp I I').*) admit. }
+          iEval (rewrite HH) in "H7 H9". iFrame "∗ % #". iPureIntro. reflexivity.
+        + iModIntro. wp_pures. wp_bind (unlockNode _)%E. 
+          iDestruct "HΦ" as "_". awp_apply (unlockNode_spec γ γ_fp γ_c n Ns'). done.
+          iSplitL. iApply "Hfp". iApply "Hin".
+          iAssert (hrep n In' ∗ own γ (◯ In') ∗ ⌜Nds In' = {[n]}⌝)%I with "[Hrep HIn' HNds]" as "Haac". { eauto with iFrame. }
+          iAaccIntro with "Haac". iIntros "(Hrep & HInt & _)". iModIntro. iFrame "Hrep". iFrame "HInt".
+          iIntros . iModIntro.  wp_pures.
+
+
+
+
+
+
+
+
+
+
+
+
+
+
+
+
+
+
+(*
+
+  Proof.
+    iIntros (Ns C). iIntros "#HInv H" (Φ) "AU". iLöb as "IH" forall (Ns).
+    wp_lam. wp_bind(traverse _ _ _)%E. iDestruct "H" as "#(H1 & H2)".
+    awp_apply (traverse_spec γ γ_fp γ_c). done. eauto with iFrame.
+    iAssert (True)%I as "Ht". done. iAaccIntro with "Ht". eauto with iFrame.
+    iIntros (n Ns' In) "(#Hin & #Hfp & HInt & Hrep & #HNds & #Hinset & #Hout)". iModIntro. wp_let.
+    wp_bind(decisiveOp dop _ _)%E. awp_apply (decisiveOp_spec dop In n k).
+    iAssert (hrep n In ∗ ⌜in_inset k In n⌝ ∗ ⌜not_in_outset k In n⌝ ∗ ⌜Nds In = {[n]}⌝)%I with "[Hrep Hinset Hout HNds]" as "Haac".
+    { eauto with iFrame. }
+    iAaccIntro with "Haac". { iIntros "(Hrep & ?)". iModIntro. iFrame. }
+    iIntros (b In' result) "Hb". destruct b; last first.
+    - iModIntro. wp_pures. awp_apply (unlockNode_spec γ γ_fp γ_c n Ns'). done. iSplit. done. iApply "Hin".
+      iAssert (hrep n In ∗ own γ (◯ In) ∗ ⌜Nds In = {[n]}⌝)%I with "[Hb HInt HNds]" as "Haac". { eauto with iFrame. }
+      iAaccIntro with "Haac". iIntros "(Hb & HInt & _)". eauto with iFrame. iIntros. iModIntro.
+      wp_pures. iApply "IH". iSplit. iApply "H1". done. done.
+    - iInv dictN as ">HI". iDestruct "HI" as (I Nd Cs) "(H3 & H4 & H5 & H6 & H7 & H8 & H9)".
+      iDestruct "H4" as %H4. iEval (rewrite H4) in "H3".
+      iPoseProof (auth_own_incl with "[$H5 $HInt]") as (I2)"%".
+      iPoseProof ((own_valid γ (● I)) with "H5") as "%".
+      iDestruct "Hb" as "(Hrep & #Hdop & Hctx & HNds')". iDestruct "Hctx" as %Hctx.
+      iMod (own_updateP (flowint_update_P I In In') γ (● I ⋅ ◯ In) with "[H5 HInt]") as (?) "H0".
+      { apply (flowint_update I In In'). admit. } { rewrite own_op. iFrame. }
+      iPoseProof ((flowint_update_result γ I In In') with "H0") as (I') "(% & % & HIIn)".
+      iAssert (own γ (● I') ∗ own γ (◯ In'))%I with "[HIIn]" as "(HI' & HIn')". { by rewrite own_op. }
+      iPoseProof ((own_valid γ (● I')) with "HI'") as "%".
+      iPoseProof ((Ψ_keyset_theorem dop k n In In' I I' result) with "[H6 HNds Hinset Hout] [Hdop]") as "HΨI".
+      { repeat iSplitL; try done; iPureIntro; apply auth_auth_valid; done. } { done. }
+      iMod "AU" as "[hoho [_ Hcl]]".
+      iDestruct (auth_agree with "H3 hoho") as %Hauth.
+      iMod (auth_update γ_c (cont I') with "H3 hoho") as "[H3 hoho]".
+      iSpecialize ("Hcl" $! (cont I') result). iEval (rewrite <-Hauth) in "Hcl".
+      iMod ("Hcl" with "[hoho HΨI]") as "HΦ". eauto with iFrame.
+      iModIntro. iSplitR "Hrep HIn' HNds HΦ".
+        + iNext. iExists I', Nd, (cont I').
+          unfold main_inv. assert (globalint I') as HI'. { (* by apply (contextualLeq_impl_globalint I I')*) admit. }
+          assert (Nds I = Nds I') as HH. { (*by apply (contextualLeq_impl_fp I I').*) admit. }
+          iEval (rewrite HH) in "H7 H9". iFrame "∗ % #". iPureIntro. reflexivity.
+        + iModIntro. wp_pures. wp_bind (unlockNode _)%E. iDestruct "HΦ" as "_". awp_apply (unlockNode_spec γ γ_fp γ_c n Ns'). done.
+          iSplitL. iApply "Hfp". iApply "Hin".
+          iAssert (hrep n In' ∗ own γ (◯ In') ∗ ⌜Nds In' = {[n]}⌝)%I with "[Hrep HIn' HNds]" as "Haac". { eauto with iFrame. }
+          iAaccIntro with "Haac". iIntros "(Hrep & HInt & _)". iModIntro. iFrame "Hrep". iFrame "HInt".
+          iIntros . iModIntro.  wp_pures.
+
+*)
+
+(*
+1) flows.contextual ...
+2) searchStrOp awp_apply (unlockNode_spec)
+3) new RA for γ_c
+
+1) new ghost location for proving disjointedness.
+*)
+
 (*
   Theorem searchStrOp_refinement dop Γ γ γ_fp γ_c (k: key) :
     is_dict γ γ_fp γ_c -∗
