coupling.v
@@ -1,0 +1,444 @@
+Add LoadPath "/home/nisarg/Academics/templates".
+From iris.algebra Require Import excl auth gmap agree gset.
+From iris.heap_lang Require Export lifting notation locations lang.
+From iris.base_logic.lib Require Export invariants.
+From iris.program_logic Require Export atomic.
+From iris.proofmode Require Import tactics.
+From iris.heap_lang Require Import proofmode notation par.
+From iris.bi.lib Require Import fractional.
+From iris.bi Require Import derived_laws_sbi.
+Require Export flows.
+Set Default Proof Using "Type*".
+
+Inductive dOp := memberOp | insertOp | deleteOp.
+
+Variable findNext : val.
+Variable decisiveOp : (dOp → val).
+Variable searchStrSpec : (dOp → val).
+Variable lockLoc : node → loc.
+Variable getLockLoc : val.
+Variable alloc : val.
+
+Variable in_inset : key → flowintUR → node → Prop.
+Variable in_edgeset : key → flowintUR → node → node → Prop.
+Variable not_in_outset : key → flowintUR → node → Prop.
+Variable cont : flowintUR → gset key.
+Variable inreach : flowintUR → node → gset key.
+Variable contextualLeq : flowintUR → flowintUR → Prop.
+Variable is_empty_flowint : flowintUR → Prop.
+
+
+Definition lockNode : val :=
+  rec: "lockN" "x" :=
+    let: "l" := getLockLoc "x" in
+    if: CAS "l" #false #true
+    then #()
+    else "lockN" "x" .
+
+Definition unlockNode : val :=
+  λ: "x",
+  let: "l" := getLockLoc "x" in
+  "l" <- #false.
+
+Definition traverse : val :=
+  rec: "tr" "p" "n" "k" :=
+    match: (findNext "n" "k") with
+      NONE => ("p", "n")
+    | SOME "n'" =>
+      lockNode "n'";; unlockNode "p";; "tr" "n" "n'" "k"
+    end.
+
+Definition searchStrOp (Ψ: dOp) (root: node) : val :=
+  rec: "dictOp" "k" :=
+    lockNode #root;;
+    match: (findNext #root "k") with
+      NONE => "dictOp" "k"  (* Need a way to modify root variable here! *)
+    | SOME "n0" =>
+      lockNode "n0";;
+      let: "pn" := traverse #root "n0" "k" in
+      let: "p" := Fst "pn" in
+      let: "n" := Snd "pn" in
+      let: "m" := alloc #() in
+      let: "res" := (decisiveOp Ψ) "p" "n" "k" in
+      unlockNode "p";; unlockNode "n";; "res"
+    end.
+
+(* ---------- Cameras used in the following proofs ---------- *)
+
+(* RA for authoritative flow interfaces *)
+Class flowintG Σ := FlowintG { flowint_inG :> inG Σ (authR flowintUR) }.
+Definition flowintΣ : gFunctors := #[GFunctor (authR flowintUR)].
+
+Instance subG_flowintΣ {Σ} : subG flowintΣ Σ → flowintG Σ.
+Proof. solve_inG. Qed.
+
+(* RA for authoritative set of nodes *)
+Class nodesetG Σ := NodesetG { nodeset_inG :> inG Σ (authR (gsetUR node)) }.
+Definition nodesetΣ : gFunctors := #[GFunctor (authR (gsetUR node))].
+
+Instance subG_nodesetΣ {Σ} : subG nodesetΣ Σ → nodesetG Σ.
+Proof. solve_inG. Qed.
+
+(* RA for set of contents *)
+Class contentG Σ := ContentG { content_inG :> inG Σ (authR (optionUR (exclR (gsetR key)))) }.
+Definition contentΣ : gFunctors := #[GFunctor (authR (optionUR (exclR (gsetR key))))].
+
+Instance subG_contentΣ {Σ} : subG contentΣ Σ → contentG Σ.
+Proof. solve_inG. Qed.
+
+Section Give_Up_Template.
+  Context `{!heapG Σ, !flowintG Σ, !nodesetG Σ, !contentG Σ} (N : namespace).
+  Notation iProp := (iProp Σ).
+
+  (* ---------- Flow interface set-up specific to this proof ---------- *)
+
+  Variable root : node.
+
+  Variable hrep : node → flowintUR → iProp.
+  Parameter hrep_timeless_proof : ∀ n I, Timeless (hrep n I).
+  Instance hrep_timeless n I : Timeless (hrep n I).
+  Proof. apply hrep_timeless_proof. Qed.
+  Parameter hrep_fp : ∀ n I_n, hrep n I_n -∗ ⌜Nds I_n = {[n]}⌝.
+
+  Variable empty_node : node → iProp.
+
+  Variable globalint : flowintUR → Prop.
+  Hypothesis globalint_root_fp : ∀ I, globalint I → root ∈ Nds I.
+  (* Hypothesis globalint_fpo : ∀ I, globalint I → FPo I = ∅. *)
+  Hypothesis globalint_root_inr : ∀ I k, globalint I → k ∈ inreach I root.
+  Hypothesis globalint_root_inset : ∀ I, globalint I → (∀ k, in_inset k I root).
+  Hypothesis globalint_add : ∀ I I' I_m,
+      globalint I → I' = I ⋅ I_m → is_empty_flowint I_m → globalint I'.
+  Hypothesis contextualLeq_impl_globalint :
+    ∀ I I', globalint I → contextualLeq I I' → globalint I'.
+
+  (* The flow graphs store keyset of region in node abstraction *)
+  (*Variable in_keyset : key → flowintUR → Prop.
+
+  Hypothesis flowint_keyset : ∀ k I_n n,
+      in_inset k I_n n ∧ not_in_outset k I_n n → in_keyset k I_n.
+  Hypothesis flowint_keyset_mono : ∀ k I1 I2, in_keyset k I1 → in_keyset k (I1 ⋅ I2).*)
+
+  (* ---------- Coarse-grained specification ---------- *)
+
+  Definition Ψ dop k (C: gsetO key) (C': gsetO key) (res: bool) : iProp :=
+    match dop with
+    | memberOp => (⌜C' = C ∧ (Is_true res ↔ k ∈ C)⌝)%I
+    | insertOp => (⌜C' = union C {[k]} ∧ (Is_true res ↔ k ∉ C)⌝)%I
+    | deleteOp => (⌜C' = difference C {[k]} ∧ (Is_true res ↔ k ∈ C)⌝)%I
+    end.
+
+  Instance Ψ_persistent dop k C C' res : Persistent (Ψ dop k C C' res).
+  Proof. destruct dop; apply _. Qed.
+
+  Lemma Ψ_determines_res dop k C1 C1' C2 C2' res1 res2 :
+    Ψ dop k C1 C1' res1 ∗ Ψ dop k C2 C2' res2 ∗ ⌜C1 = C2⌝ -∗ ⌜res1 = res2⌝.
+  Proof.
+    destruct dop; iPureIntro; destr_bool;
+      destruct H as ((HC1 & HkC1) & (HC2 & HkC2) & HEq);
+      exfalso; rewrite HEq in HkC1; rewrite <- HkC2 in HkC1; inversion HkC1;
+        contradiction.
+  Qed.
+
+  Lemma Ψ_determines_C' dop k C1 C1' C2 C2' res1 res2 :
+    Ψ dop k C1 C1' res1 ∗ Ψ dop k C2 C2' res2 ∗ ⌜C1 = C2⌝ -∗ ⌜C1' = C2'⌝.
+  Proof.
+    destruct dop; iPureIntro; simpl; destr_bool;
+      destruct H as ((HC1 & HkC1) & (HC2 & HkC2) & HEq); congruence.
+  Qed.
+
+  Axiom Ψ_keyset_theorem : ∀ (dop: dOp) (k: key) (n: node) (I_n I_n' I I': flowintUR) (res: bool),
+      ⌜globalint I⌝ ∗ ⌜Nds I_n = {[n]}⌝ ∗ ⌜in_inset k I_n n⌝ ∗ ⌜not_in_outset k I_n n⌝
+      ∗ ⌜(∃ (I_o: flowintUR), I = I_n ⋅ I_o ∧ I' = I_n' ⋅ I_o)⌝ ∗ ✓ I ∗ ✓ I'
+      -∗ Ψ dop k (cont I_n) (cont I_n') res -∗ Ψ dop k (cont I) (cont I') res.
+
+  (* ---------- Helper functions specs - proved for each implementation in GRASShopper ---------- *)
+
+  Parameter getLockLoc_spec : ∀ (n: node),
+                  (<<< True >>> getLockLoc #n @ ⊤
+                           <<< ∃ l:loc, ⌜lockLoc n = l⌝, RET #l >>>)%I.
+
+  Parameter findNext_spec : ∀ (n: node) (I_n : flowintUR) (k: key),
+                  (<<< hrep n I_n >>> findNext #n #k @ ⊤
+                              <<< ∃ (b: bool) (n': node), hrep n I_n ∗ (match b with true => ⌜in_edgeset k I_n n n'⌝ |
+                                                                                     false => ⌜not_in_outset k I_n n⌝ end),
+                                  RET (match b with true => (SOMEV #n') | 
+                                                    false => NONEV end) >>>)%I.
+
+  Parameter decisiveOp_3_spec : ∀ (dop: dOp) (I_p I_n I_m: flowintUR) (p n m: node) (k:key),
+                  (<<< hrep p I_p ∗ hrep n I_n ∗ empty_node m ∗ ⌜is_empty_flowint I_m ⌝ ∗ ⌜Nds I_m = {[m]}⌝ 
+                          ∗ ⌜✓I_m⌝ ∗ ⌜in_edgeset k I_p p n⌝ ∗ ⌜in_inset k I_n n⌝ ∗ ⌜not_in_outset k I_n n⌝ >>>
+                             decisiveOp dop #p #n #k @ ⊤
+                    <<< ∃ (b: bool) (I_p' I_n' I_m': flowintUR) (res: bool), 
+                          match b with false => hrep p I_p ∗ hrep n I_n ∗ empty_node m 
+                                                  ∗ Ψ dop k (cont (I_p ⋅ I_n)) (cont (I_p ⋅ I_n)) res |
+                                        true => hrep p I_p' ∗ hrep n I_n' ∗ hrep m I_m'
+                                                ∗ Ψ dop k (cont (I_p ⋅ I_n ⋅ I_m)) (cont (I_p' ⋅ I_n' ⋅ I_m')) res
+                                                ∗ ⌜Nds I_p' = {[p]}⌝ ∗ ⌜Nds I_n' = {[n]}⌝ ∗ ⌜Nds I_m' = {[m]}⌝
+                                                ∗ ⌜contextualLeq (I_p ⋅ I_n ⋅ I_m) (I_p' ⋅ I_n' ⋅ I_m')⌝ end,
+                          RET #res >>>)%I.
+
+
+
+  (* ---------- The invariant ---------- *)
+
+  Definition dictN : namespace := N .@ "dict".
+
+  Definition main_inv (γ: gname) (γ_fp: gname) (γ_c: gname) I Ns C
+    : iProp :=
+    (own γ_c (● (Some (Excl C))) ∗ ⌜C = cont I⌝
+        ∗ own γ (● I) ∗ ⌜globalint I⌝
+        ∗ ([∗ set] n ∈ (Nds I), (∃ b: bool, (lockLoc n) ↦ #b
+                                ∗ if b then True else (∃ (In: flowintUR),
+                                                         own γ (◯ In) ∗ hrep n In ∗ ⌜Nds In = {[n]}⌝)))
+        ∗ own γ_fp (● Ns) ∗ ⌜Ns = (Nds I)⌝
+    )%I.
+
+  Definition is_dict γ γ_fp γ_c :=
+    inv dictN (∃ I Ns C, (main_inv γ γ_fp γ_c I Ns C))%I.
+
+  Instance main_inv_timeless γ γ_fp γ_c I N C :
+    Timeless (main_inv γ γ_fp γ_c I N C).
+  Proof.
+    rewrite /main_inv. repeat apply bi.sep_timeless; try apply _.
+    try apply big_sepS_timeless. intros. apply bi.exist_timeless. intros.
+    apply bi.sep_timeless; try apply _.
+    destruct x0; try apply _.
+  Qed.
+
+  (* ---------- Assorted useful lemmas ---------- *)
+
+  Lemma auth_set_incl γ_fp Ns Ns' :
+    own γ_fp (◯ Ns) ∗ own γ_fp (● Ns') -∗ ⌜Ns ⊆ Ns'⌝.
+  Proof.
+    rewrite -own_op. rewrite own_valid. iPureIntro.
+    rewrite auth_valid_discrete. simpl. rewrite ucmra_unit_right_id_L.
+    intros. destruct H. inversion H0 as [m H1].
+    destruct H1. destruct H2. apply gset_included in H2. rewrite /to_agree in H1.
+    Admitted.
+
+  Lemma auth_own_incl γ (x y: flowintUR) : own γ (● x) ∗ own γ (◯ y) -∗ ⌜y ≼ x⌝.
+  Proof.
+    rewrite -own_op. rewrite own_valid. iPureIntro. rewrite auth_valid_discrete.
+    simpl. rewrite ucmra_unit_left_id_L. Admitted.
+
+  Lemma auth_agree γ xs ys :
+    own γ (● (Excl' xs)) -∗ own γ (◯ (Excl' ys)) -∗ ⌜xs = ys⌝.
+  Proof.
+   iIntros "Hγ● Hγ◯". by iDestruct (own_valid_2 with "Hγ● Hγ◯")
+      as %[<-%Excl_included%leibniz_equiv _]%auth_both_valid.
+  Qed.
+
+  (** The view of the authority can be updated together with the local view. *)
+  Lemma auth_update γ ys xs1 xs2 :
+    own γ (● (Excl' xs1)) -∗ own γ (◯ (Excl' xs2)) ==∗
+      own γ (● (Excl' ys)) ∗ own γ (◯ (Excl' ys)).
+  Proof.
+    iIntros "Hγ● Hγ◯".
+    iMod (own_update_2 _ _ _ (● Excl' ys ⋅ ◯ Excl' ys)
+      with "Hγ● Hγ◯") as "[$$]".
+    { by apply auth_update, option_local_update, exclusive_local_update. }
+    done.
+  Qed.
+
+
+  Lemma flowint_update_result γ I I_n I_n' x :
+    ⌜flowint_update_P I I_n I_n' x⌝ ∧ own γ x -∗
+                                          ∃ I', ⌜contextualLeq I I'⌝ ∗ ⌜∃ I_o, I = I_n ⋅ I_o ∧ I' = I_n' ⋅ I_o⌝ 
+                                                                     ∗ own γ (● I' ⋅ ◯ I_n').
+  Proof.
+    unfold flowint_update_P. simpl.
+    case_eq (auth_auth_proj x); last first.
+    - intros H. iIntros "(% & ?)". iExFalso. done.
+    - intros p. intros H. case_eq p. intros q a Hp. case_eq a.
+      intros intl b Ha. destruct intl as [ | I' ?]. iIntros "(% & ?)". iExFalso. done.
+      case_eq intl; last first. intros u0 l _. iIntros "(% & ?)". iExFalso. done.
+      + intros Hintl. simpl in b. assert (b = eq_refl) as H0. { admit. }
+        rewrite H0. iIntros "(Hfr & Hown)". iDestruct "Hfr" as %Hfr. destruct Hfr as [Hfrag Hcon].
+        destruct Hcon as [Hcon HIo]. destruct HIo as [Io HIo]. iExists I'.
+        iSplitR. iPureIntro. { admit. }
+        iSplitR. iPureIntro. exists Io. done.
+  Admitted.
+
+  Parameter alloc_spec : ∀ γ γ_fp γ_c,
+        is_dict γ γ_fp γ_c -∗ 
+                <<< True >>> alloc #() @ ⊤∖↑dictN
+                <<< ∃ (m: node) (I_m: flowintUR), empty_node m ∗ own γ (◯ I_m) ∗ ⌜Nds I_m = {[m]}⌝ 
+                                                ∗ ⌜✓I_m⌝ ∗ ⌜is_empty_flowint I_m⌝, RET #m >>>.
+
+  (* ---------- Ghost state manipulation to make final proof cleaner ---------- *)
+
+  Lemma ghost_update_step γ γ_fp γ_c (n n': node) (k:key) (Ns: gset node) (I_n: flowintUR):
+          is_dict γ γ_fp γ_c -∗ own γ (◯ I_n) ∗ ⌜Nds I_n = {[n]}⌝∗ ⌜in_inset k I_n n⌝ ∗ ⌜in_edgeset k I_n n n'⌝ 
+                                ={ ⊤ }=∗ ∃ (Ns': gset node), own γ_fp (◯ Ns') ∗ ⌜n' ∈ Ns'⌝ ∗ ⌜n ∈ Ns'⌝ ∗ own γ (◯ I_n) ∗ ⌜root ∈ Ns'⌝.
+  Proof.
+  Admitted.
+
+  Lemma ghost_update_step_2 γ γ_fp γ_c (n n': node) (k:key) (Ns: gset node) (I_n I_n': flowintUR):
+          is_dict γ γ_fp γ_c -∗ own γ (◯ I_n) ∗ ⌜Nds I_n = {[n]}⌝ ∗ own γ (◯ I_n') ∗ ⌜Nds I_n' = {[n']}⌝
+          ∗ ⌜in_inset k I_n n⌝ ∗ ⌜in_edgeset k I_n n n'⌝ ={ ⊤ }=∗ own γ (◯ I_n) ∗ own γ (◯ I_n') ∗ ⌜in_inset k I_n' n'⌝.
+  Proof.
+  Admitted.
+
+  Lemma ghost_update_root_inset γ γ_fp γ_c (k:key) (I_root: flowintUR):
+          is_dict γ γ_fp γ_c -∗ own γ (◯ I_root) ∗ ⌜Nds I_root = {[root]}⌝ 
+                                ={ ⊤ }=∗ own γ (◯ I_root) ∗ ⌜in_inset k I_root root⌝.
+  Proof.
+  Admitted.
+
+  Lemma ghost_update_root_fp γ γ_fp γ_c :
+          is_dict γ γ_fp γ_c -∗ True
+                                ={ ⊤ }=∗ ∃ (Ns: gsetUR node), own γ_fp (◯ Ns) ∗ ⌜root ∈ Ns⌝.
+  Proof.
+  Admitted.
+
+  (* ---------- Lock module proofs ---------- *)
+
+  Lemma lockNode_spec (γ: gname) (γ_fp: gname) (γ_c: gname) (n: node) (Ns: gset node):
+    is_dict γ γ_fp γ_c -∗ own γ_fp (◯ Ns) ∗ ⌜n ∈ Ns⌝ -∗
+          <<< True >>>
+                lockNode #n    @ ⊤ ∖ ↑dictN
+          <<< ∃ (I_n: flowintUR), own γ (◯ I_n) ∗ hrep n I_n ∗ ⌜Nds I_n = {[n]}⌝, RET #() >>>.
+  Proof.
+    iIntros "#HInv [Hl1 Hl2]" (Φ) "AU". iLöb as "IH".
+    wp_lam. awp_apply getLockLoc_spec.
+    iAssert (True)%I as "Ht". done.
+    iAaccIntro with "Ht". eauto 4 with iFrame.
+    iIntros (l) "#Hl". iModIntro. wp_let. wp_bind (CmpXchg _ _ _)%E.
+    iInv dictN as ">HI".
+    iDestruct "HI" as (I' N' C') "(H1 & H2 & H3 & H4 & H5 & H6 & H7)". iDestruct "Hl" as %Hl.
+    iAssert (⌜n ∈ Nds I'⌝)%I with "[Hl1 Hl2 H6 H7]" as "%".
+    { (*iEval (rewrite <- H1).*) iPoseProof ((auth_set_incl γ_fp Ns N') with "[$]") as "%".
+      iDestruct "H7" as %H7. iDestruct "Hl2" as %Hl2. iEval (rewrite <-H7). iPureIntro. set_solver. }
+    rewrite (big_sepS_elem_of_acc _ (Nds I') n); last by eauto.
+    iDestruct "H5" as "[ho hoho]".
+    iDestruct "ho" as (b) "[Hlock Hlock']". iEval (rewrite Hl) in "Hlock". destruct b.
+      - wp_cmpxchg_fail. iModIntro. iSplitR "Hl1 Hl2 AU". iNext. iExists I', N', C'. iFrame. iApply "hoho".
+        iExists true. iEval (rewrite <-Hl) in "Hlock". iSplitL "Hlock". done. done. wp_pures.
+        iDestruct "Hl1" as "#Hl1". iDestruct "Hl2" as "#Hl2". iApply "IH". done. done. done.
+      - iMod "AU" as "[Ht [_ Hcl]]". iDestruct "Hlock'" as (In) "hehe".
+        wp_cmpxchg_suc. iMod ("Hcl" with "hehe") as "HΦ".
+        iModIntro. iModIntro. iSplitR "HΦ".
+          * iNext. iExists I', N', C'. rewrite /main_inv. iFrame.
+                iApply "hoho". iExists true. iEval (rewrite <-Hl) in "Hlock". iFrame.
+          * wp_pures. done.
+  Qed.
+
+  Lemma unlockNode_spec (γ: gname) (γ_fp: gname) (γ_c: gname) (n: node) (Ns: gset node) :
+    is_dict γ γ_fp γ_c -∗ own γ_fp (◯ Ns) ∗ ⌜n ∈ Ns⌝ -∗
+          <<< ∀ (I_n: flowintUR), hrep n I_n ∗ own γ (◯ I_n) ∗ ⌜Nds I_n = {[n]}⌝ >>>
+                unlockNode #n    @ ⊤ ∖ ↑dictN
+          <<< True, RET #() >>>.
+  Proof.
+    iIntros "#Hinv (Hfp & Hin)" (Φ) "AU". wp_lam. awp_apply getLockLoc_spec.
+    iAssert (True)%I as "Ht". done.
+    iAaccIntro with "Ht". eauto 4 with iFrame.
+    iIntros (l) "Hl". iDestruct "Hl" as %Hl. iModIntro. wp_let. iInv dictN as ">HI".
+    iDestruct "HI" as (I' N' C') "(H1 & H2 & H3 & H4 & H5 & H6 & H7)".
+    iAssert (⌜n ∈ Nds I'⌝)%I with "[Hfp Hin H6 H7]" as "%".
+    { (*iEval (rewrite <- H1).*) iPoseProof ((auth_set_incl γ_fp Ns N') with "[$]") as "%".
+      iDestruct "H7" as %H7. iDestruct "Hin" as %Hl2. iEval (rewrite <-H7). iPureIntro. set_solver. }
+    rewrite (big_sepS_elem_of_acc _ (Nds I') n); last by eauto.
+    iDestruct "H5" as "[ho hoho]".
+    iDestruct "ho" as (b) "[Hlock Hlock']".
+    iEval (rewrite Hl) in "Hlock".
+    iMod "AU" as (I_n) "[Hr [_ Hcl]]". wp_store.
+    iAssert (True)%I as "Ht". done.
+    iMod ("Hcl" with "Ht") as "HΦ".
+    iModIntro. iModIntro. iSplitR "HΦ". iNext. iExists I', N', C'. rewrite /main_inv. iFrame.
+    iApply "hoho". iExists false. iEval (rewrite <-Hl) in "Hlock". iFrame. iExists I_n. 
+    iDestruct "Hr" as "(? & ? & ?)". eauto with iFrame. done.
+  Qed.
+
+  (* ---------- Refinement proofs ---------- *)
+
+  Lemma traverse_spec γ γ_fp γ_c (I_p I_n: flowintUR) (Ns: gset node) (p n: node) (k: key) :
+    is_dict γ γ_fp γ_c -∗ hrep n I_n ∗ own γ (◯ I_n) ∗ ⌜Nds I_n = {[n]}⌝ ∗ ⌜in_inset k I_n n⌝
+                          ∗ own γ_fp (◯ Ns) ∗ ⌜p ∈ Ns⌝ ∗ ⌜n ∈ Ns⌝ ∗ own γ (◯ I_p) 
+                          ∗ hrep p I_p ∗ ⌜Nds I_p = {[p]}⌝ ∗ ⌜in_edgeset k I_p p n⌝ -∗
+        <<< True >>>
+                  traverse #p #n #k @ ⊤∖↑dictN
+        <<< ∃ (p' n': node) (I_p' I_n': flowintUR), own γ (◯ I_p') ∗ own γ (◯ I_n') ∗ hrep p' I_p' ∗ hrep n' I_n'
+                                          ∗ ⌜Nds I_p' = {[p']}⌝ ∗ ⌜Nds I_n' = {[n']}⌝ ∗ ⌜in_edgeset k I_p' p' n'⌝
+                                          ∗ ⌜in_inset k I_n' n'⌝ ∗ ⌜not_in_outset k I_n' n'⌝,
+              RET (#p', #n') >>>.
+  Proof.
+    iIntros "#Hinv H". iLöb as "IH" forall (p n Ns I_p I_n). iIntros (Φ) "AU".
+    iDestruct "H" as "(Hrep & HIn & #HNdsN & #Hinset & #HNs & #HinP & #HinN & HIp & HrepP & #HNdsP & #Hedge)".
+    wp_lam. wp_let. wp_let. wp_bind (findNext _ _)%E.
+    awp_apply (findNext_spec n I_n k).
+    iAaccIntro with "Hrep". eauto with iFrame.
+    iIntros (b n') "(Hrep & Hb)". destruct b; last first.
+    - iMod "AU" as "[Ht [_ HClose]]".
+      iSpecialize ("HClose" $! p n I_p I_n).
+      iMod ("HClose" with "[HIp HIn HrepP Hrep HNdsP HNdsN Hedge Hinset Hb]") as "HΦ".
+      { eauto with iFrame. }
+      iModIntro. wp_match. wp_pures. done.
+    - iDestruct "Hb" as "#Hb".
+      iDestruct (ghost_update_step γ γ_fp γ_c n n' k Ns I_n with "[Hinv] [HIn HNdsN Hinset Hb]") as ">HN".
+      done. eauto with iFrame. iDestruct "HN" as (Ns')"(#HNs' & #Hin' & #Hin & HIn & #Hroot)".
+      iModIntro. wp_pures. awp_apply (lockNode_spec γ γ_fp γ_c n' Ns'). done. eauto with iFrame.
+      iAssert (True)%I as "Ht". { done. } iAaccIntro with "Ht". eauto with iFrame.
+      iIntros (I_n') "(HIn' & Hrep' & #HNds')". iModIntro. wp_pures.
+      awp_apply (unlockNode_spec γ γ_fp γ_c p Ns). done. eauto with iFrame.
+      iAssert (hrep p I_p ∗ own γ (◯ I_p) ∗ ⌜Nds I_p = {[p]}⌝)%I with "[HrepP HIp HNdsP]" as "Haac". { eauto with iFrame. }
+      iAaccIntro with "Haac". iIntros "(HrepP & HIp & _)". iModIntro. eauto with iFrame.
+      iIntros. iModIntro. wp_pures. iSpecialize ("IH" $! n n' Ns' I_n I_n').
+      iDestruct (ghost_update_step_2 γ γ_fp γ_c n n' k Ns I_n I_n' with "[Hinv] [HIn HNdsN HIn' HNds' Hinset Hb]") as ">HN".
+      { done. } { eauto with iFrame. } iDestruct "HN" as "(HIn & HIn' & #Hb')".
+      iApply ("IH" with "[Hrep' HIn' HNds' HIn Hrep]"). 
+      { iSplitL "Hrep'". done. iSplitL "HIn'". done.  
+        iSplitL "HNds'". done. iSplitL "Hb'". done.
+        iSplitL "HNs'". done. iSplitL "Hin". done.
+        iSplitL "Hin'". done. iSplitL "HIn". done.
+        eauto with iFrame. } done.
+  Qed.
+
+  Theorem searchStrOp_spec (γ γ_fp γ_c: gname) (dop: dOp) (k: key):
+          ∀ (Ns: gsetUR node) (C: gset key),
+          is_dict γ γ_fp γ_c -∗ own γ_fp (◯ Ns) ∗ ⌜ root ∈ Ns ⌝ -∗
+      <<< own γ_c (◯ (Some (Excl C))) >>>
+            (searchStrOp dop root) #k
+                  @ ⊤∖↑dictN
+      <<< ∃ (C': gset key) (res: bool), own γ_c (◯ (Some (Excl C'))) ∗ ⌜Ψ dop k C C' res⌝, RET #res >>>.
+  Proof.
+    iIntros (Ns C). iIntros "#HInv H" (Φ) "AU". iLöb as "IH".
+    iDestruct "H" as "#(Hfp & Hroot)". wp_lam. wp_bind(lockNode _)%E.
+    awp_apply (lockNode_spec γ γ_fp γ_c root Ns). done. eauto with iFrame.
+    iAssert (True)%I as "#Ht". { done. } iAaccIntro with "Ht". eauto with iFrame.
+    iIntros (Ir) "(HIr & HrepR & #HNdsR)". iModIntro. wp_pures.
+    wp_bind (findNext _ _)%E. awp_apply (findNext_spec root Ir k).
+    iAaccIntro with "HrepR". eauto with iFrame.
+    iIntros (b n) "(HrepR & Hb)". destruct b; last first.
+    - iModIntro. wp_pures. iApply "IH". iFrame "Hfp Hroot". done.
+    - iModIntro. wp_pures. wp_bind (lockNode _)%E. iDestruct "Hb" as "#Hb".
+      iDestruct (ghost_update_root_inset γ γ_fp γ_c k Ir with "[HInv] [HIr HNdsR]") as ">HN".
+      done. eauto with iFrame. iDestruct "HN" as "(HIr & #HinsetR)".
+      iDestruct (ghost_update_step γ γ_fp γ_c root n k Ns Ir with "[HInv] [HIr HNdsR Hb HinsetR]") as ">HN".
+      done. eauto with iFrame. iDestruct "HN" as (Ns') "(#Hfp' & #HinN & #HinR & HIr & _)".
+      awp_apply (lockNode_spec γ γ_fp γ_c n Ns'). done. eauto with iFrame.
+      iAaccIntro with "Ht". eauto with iFrame.
+      iIntros (In) "(HIn & HrepN & #HNdsN)". iModIntro. wp_pures.
+      wp_bind (traverse _ _ _)%E.
+      iDestruct (ghost_update_step_2 γ γ_fp γ_c root n k Ns' Ir In with "[HInv] [HIr HNdsR HIn HNdsN HinsetR Hb]") as ">HN".
+      done. eauto with iFrame. iDestruct "HN" as "(HIr & HIn & #HinsetN)".
+      awp_apply (traverse_spec γ γ_fp γ_c Ir In Ns' root n k with "[] [HIr HIn HrepR HrepN]") . done.
+      iFrame "HrepN HIn HNdsN HinsetN Hfp' HinR HinN HIr HrepR HNdsR Hb".
+      iAaccIntro with "Ht". eauto with iFrame.
+      iIntros (p' n' Ip' In') "(HIp' & HIn' & HrepP' & HrepN' & #HNdsP' & #HNdsN' & #HedgeP' & #HinsetN' & #HnotoutN')".
+      iModIntro. wp_pures. wp_bind(alloc _)%E. awp_apply (alloc_spec γ γ_fp γ_c). done.
+      iAaccIntro with "Ht". eauto with iFrame.
+      iIntros (m Im) "(HempM & HIm & #HNdsM & #HM & #HempIntM)".
+      iModIntro. wp_pures. wp_bind (decisiveOp _ _ _ _)%E. iDestruct "HempM" as "_".
+      awp_apply (decisiveOp_3_spec dop Ip' In' Im p' n' m k).
+
+
+(* 
+1) 2 issues in give-up.
+2) no funding for popl
+3) can use ghost_step and change the preconditions.
+*)
+
+
+
+
